library/widget/examples.lean
@@ -1,7 +1,7 @@
-open html
-open html.attr
-
-namespace component
+/- Author: E.W.Ayers
+Some components for testing and as examples.
+ -/
+namespace widget
 
 meta class has_show_html (π : Type) :=
 (show_html' {α : Type}: π → html α)
@@ -20,27 +20,29 @@ component.mk π π
 (λ ⟨⟩ x, has_to_editor.comp x)
 
 meta instance string_editor : has_to_editor string :=
-⟨λ s, html.textbox s (λ s', s')⟩
+⟨λ s, textbox s (λ s', s')⟩
+
+namespace examples
 
 /-- An example component which makes a 'like button'. One of the first examples from react. -/
 meta def example_like_widget : component unit empty :=
 -- trace "this is making a widget happen" $
 component.mk unit bool (λ _ _, ff) (λ _ s b, (tt, none)) (λ _ s,
   if s then "you liked this!" else
-  html.h "div" [] [html.of_string "here is a comment ", button "like this" ()]
+  h "div" [] [html.of_string "here is a comment ", button "like this" ()]
 )
 
 /-- A simple counter that can be incremented or decremented with some buttons. -/
 meta def counter_widget {π α : Type} : component π α :=
 component.mk int int (λ p x, 0 <| x) (λ _ x y, (x + y, none)) (λ _ s,
-  html.h "div" [] [
+  h "div" [] [
     button "+" (1 : int),
-    of_string $ to_string $ s,
+    html.of_string $ to_string $ s,
     button "-" (-1)
   ]
 )
 
-meta def with_hover {π α : Type} (tooltip : π → html α) (elt : π → element α) : component π α :=
+meta def with_hover {π α : Type} (tooltip : π → html α) (elt : π → html α) : component π α :=
 component.mk (bool ⊕ α) bool
   (λ props prev, ff <| prev)
   (λ props state event,
@@ -49,13 +51,13 @@ component.mk (bool ⊕ α) bool
     | (sum.inr a) := (state, some a)
     end)
   (λ props state,
-    let elt : element (bool ⊕ α) := element.map_action sum.inr $ elt props in
-    let atrs : list (attr (bool ⊕ α)) := [attr.on_mouse_enter (λ _, sum.inl tt), attr.on_mouse_leave (λ _, sum.inl ff)] in
+    let elt : html (bool ⊕ α) := html.map_action sum.inr $ elt props in
+    let atrs : list (attr (bool ⊕ α)) := [on_mouse_enter (λ _, sum.inl tt), on_mouse_leave (λ _, sum.inl ff)] in
     [
       if state then
-        html.of_element $ element.with_attrs atrs elt
+        with_attrs atrs elt
       else
-        html.of_element $ element.with_attrs ((attr.tooltip $ html.map_action sum.inr $ tooltip props) :: atrs) elt
+        with_attrs ((attr.tooltip $ html.map_action sum.inr $ tooltip props) :: atrs) elt
     ])
 
 
@@ -64,20 +66,6 @@ component.mk (bool ⊕ α) bool
 -- ⟨component.filter_map_action (λ a, none)⟩
 -- meta instance component_of_no_action {π α : Type}: has_coe (component unit α) (component π α) :=
 -- ⟨λ c, component.map_action (λ (o : empty), empty.rec (λ _, α) o) $ component.map_props (λ p, ()) $ c⟩
-
-meta def initial_action {π α : Type} : component π α → component π empty
-| c := component.filter_map_action (λ a, none) c
-
-meta def terminal_props {π α : Type} : component unit α → component π α
-| c := component.map_props (λ p, ()) $ c
-
-
-meta def aligned_list {α} (rows : list (list (html α))) : html α :=
-h "div" [className "mw6"] $ rows.map (λ r,
-  h "div" [className "dt w-100 pb2"] $ r.map (λ c,
-    with_classname "dtc v-mid" c
-  )
-)
 
 meta def dotted_border_list {α β : Type} (get_key : β → string) (view : β → html α ) : list β → html α | l :=
 h "div" [className "pa3 pa5-ns"] [
@@ -91,8 +79,7 @@ inductive todo_list_action (α : Type)
 | insert : α → todo_list_action
 | delete : nat → todo_list_action
 
-meta def todo_list (α : Type) [inhabited α] [has_show_html α] [has_to_editor α] : list α → component unit empty
-| initial :=
+meta def todo_list (α : Type) [inhabited α] [has_show_html α] [has_to_editor α] (initial : list α) : component unit empty :=
   let starts := initial.mapi (λ a i, (i, a)) in
   component.mk (todo_list_action α) (nat × list (nat × α))
   (λ _ x, ⟨starts.length, starts⟩ <| x )
@@ -103,7 +90,7 @@ meta def todo_list (α : Type) [inhabited α] [has_show_html α] [has_to_editor 
     end
   )
   (λ ⟨⟩ ⟨i,items⟩,
-    [ html.h "div" [className "mw6"] $
+    [ h "div" [className "mw6"] $
       items.map (λ ⟨k,a⟩,
         h "div" [className "flex justify-between items-center w-100 bb b--black-20 pb2 mt2", key k] [
           h "div" [className "dtc v-mid"] [show_html a],
@@ -111,53 +98,41 @@ meta def todo_list (α : Type) [inhabited α] [has_show_html α] [has_to_editor 
             className "dtc v-mid f6 button-reset bg-white ba b--black-20 dim pointer pv1 w2",
             on_click (λ _, todo_list_action.delete $ k)] ["x"]
         ]
-      )
-      ++ [
-        h "hr" [] [],
-        h "div" [className "flex justify-between items-center w-100 bb b--black-20 pb2 mt2", key "add row"] [
-          html.map_action (λ x, todo_list_action.insert x)
-          $ html.of_component ()
-          $ @component.mk α unit (option α) α
-          (λ ⟨⟩ prev, inhabited.default α <| prev)
-          (λ ⟨⟩ x b, match b with none := (inhabited.default α, some x) | (some x') := (x', none) end)
-          (λ ⟨⟩ x, [
-            h "div" [className "dtc v-mid"] [
-              html.map_action some $ has_to_editor.comp x
-            ],
-            h "button" [
-              className "dtc v-mid f6 button-reset bg-white ba b--black-20 dim pointer pv1 w2",
-              on_click (λ _, none)] ["+"]
-          ])
-        ]
-      ]
-    ]
-)
+      ) ++  [ h "hr" [] []
+            , h "div" [className "flex justify-between items-center w-100 bb b--black-20 pb2 mt2", key "add row"]
+                [ html.map_action (λ x, todo_list_action.insert x)
+                  $ html.of_component ()
+                  $ @component.mk unit α (option α) α
+                      (λ ⟨⟩ prev, inhabited.default α <| prev)
+                      (λ ⟨⟩ x b, match b with none := (inhabited.default α, some x) | (some x') := (x', none) end)
+                      (λ ⟨⟩ x,  [ h "div" [className "dtc v-mid"]
+                                    [html.map_action some $ has_to_editor.comp x]
+                                , h "button"
+                                    [className "dtc v-mid f6 button-reset bg-white ba b--black-20 dim pointer pv1 w2"
+                                    , on_click (λ _, none)]
+                                    ["+"]
+                                ])]]])
 
 meta def simple_tooltip_component : component tactic_state empty :=
 component.stateless (λ _, [
   h "div" [
     className "grow dib bg-pink black-90 pa5",
-    tooltip (
+    attr.tooltip (
       h "div" [className "pa3 bg-light-blue"] ["this is the tooltip content"]
-    )
-    ] ["this is some text with a tooltip"]
+    )] ["this is some text with a tooltip"]
 ])
-
--- meta def fake_todo_list (α : Type) : component unit empty :=
--- component.mk (todo_list_action α) (nat)
--- (λ _ _, 0)
--- (λ _ _ _, (4, none))
--- (λ _ _, ["hello world"])
 
 meta def string_todo_list : component tactic_state string :=
 component.map_action (λ (o : empty), empty.rec (λ _, _) o) $ component.map_props (λ p, ()) $
 todo_list string ["make some tasks", "delete some tasks"]
 
-
+/-- Performs a simple editor action for testing insertion to sourcetext. -/
 meta def simple_action (cmd : string) : component tactic_state string :=
 component.mk unit nat
 (λ _ _, 0)
 (λ _ n _, (n+1, some (cmd ++ to_string n)))
-(λ _ n, [html.button ("add " ++ cmd ++ to_string n) ()])
+(λ _ n, [button ("add " ++ cmd ++ to_string n) ()])
 
-end component
+end examples
+
+end widget
