tests/lean/inst.lean
@@ -6,10 +6,10 @@ class inductive C (A : Type*)
 definition val {A : Type*} (c : C A) : A :=
 C.rec (λa, a) c
 
-constant magic (A : Type*) : A
+constant wizard (A : Type*) : A
 attribute [instance, priority std.priority.max]
-noncomputable definition C_magic (A : Type*) : C A :=
-C.mk (magic A)
+noncomputable definition C_wizard (A : Type*) : C A :=
+C.mk (wizard A)
 
 attribute [instance]
 definition C_prop : C Prop :=
@@ -19,7 +19,7 @@ attribute [instance]
 definition C_prod {A B : Type*} (Ha : C A) (Hb : C B) : C (prod A B) :=
 C.mk (prod.mk (val Ha) (val Hb))
 
--- C_magic will be used because it has max priority
+-- C_wizard will be used because it has max priority
 noncomputable definition test : C (prod Prop Prop) :=
 by tactic.apply_instance
 
