tests/lean/interactive/widget1.lean
@@ -2,15 +2,16 @@ import widget
 
 example {P Q : Prop} : P → Q → P ∧ Q :=
 begin [widget_tactic]
-  put (component.string_todo_list),
+  put (widget.examples.string_todo_list),
   tactic.intros,
   tactic.split,
   tactic.assumption, tactic.assumption,
 end
 
 example {P Q : Prop} : P → Q → P ∧ Q :=
-begin [widget_tactic]
+begin
   tactic.intros,
   tactic.split,
-  tactic.assumption, tactic.assumption,
+  tactic.assumption,
+  tactic.assumption,
 end
