tests/lean/interactive/widget2.lean
@@ -2,7 +2,7 @@ import widget
 
 example {P Q : Prop} : P → Q → P ∧ Q :=
 begin [widget_tactic]
-  put (component.counter_widget),
+  put (widget.examples.counter_widget),
   tactic.intros,
   tactic.split,
   tactic.assumption, tactic.assumption,
